proof/schnorr_protocol/W64_SchnorrProtocol.ec
@@ -1,6 +1,6 @@
 require import Int Real Distr.
 require import JModel JBigNum Array32 Array64 Array128.
-require import ZK_SchnorrBasics.
+require import Ring_ops_proof ZK_SchnorrBasics.
 
 
 require export W64_SchnorrProver W64_SchnorrVerifier.
