proof/schnorr_protocol/ZK_SchnorrExtractability.ec
@@ -4,7 +4,7 @@ require import AllCore DBool Bool List Distr AuxResults Finite.
 require import ZK_SchnorrBasics.
 require import ZK_SchnorrSpecialSoundness.
 
-require import Ring_ops_spec.
+require import Ring_ops_spec Ring_ops_proof.
 import Zp.
 
 section.
